sorted theorem for insert sort refactored

insertion-sort.thy
@@ -4,20 +4,29 @@ begin
 
 declare[[names_short]]
 
-fun insert_a:: "nat \<Rightarrow> nat list \<Rightarrow> nat list" where
-insert_a_Nil: "insert_a x [] = [x]" |
-insert_a_Cons: "insert_a x (y#ys) = (if x \<le> y then (x#y#ys) else y#insert_a x ys)"
+fun insert:: "nat \<Rightarrow> nat list \<Rightarrow> nat list" where
+insert_Nil: "insert x [] = [x]" |
+insert_Cons: "insert x (y#ys) = (if x \<le> y then (x#y#ys) else y#insert x ys)"
 
-value "insert_a 1 [2,4,10]"
+value "insert 1 [2,4,10]"
 
 fun insert_sort:: "nat list \<Rightarrow> nat list" where
 insert_sort_Nil : "insert_sort []  = []" |
-insert_sort_Cons: "insert_sort (x#xs)  = insert_a x (insert_sort(xs))"
+insert_sort_Cons: "insert_sort (x#xs)  = insert x (insert_sort(xs))"
 
 value "insert_sort [2,4,10,0,3]"
 
-lemma p_1 : "sorted(ys) \<Longrightarrow> sorted (insert_a x ys)"
-proof (induct ys rule: insert_a.induct)
+lemma p_19999 : "\<lbrakk>sorted(y#ys); \<not> x \<le> y\<rbrakk> \<Longrightarrow> sorted (y#insert x ys)"
+proof(induction ys arbitrary: y rule: sorted.induct)
+  case 1
+  then show ?case by auto
+next
+  case (2 x ys)
+  then show ?case by (metis insert_Cons le_cases sorted2)
+qed
+
+lemma p_1 : "sorted(ys) \<Longrightarrow> sorted (insert x ys)"
+proof (induct ys rule: insert.induct)
   case (1 x)
   then show ?case by simp
 next
@@ -27,36 +36,32 @@ next
     case True
     have "sorted (y#ys)" using "local.2.prems" by blast
     also have "sorted (x#y#ys)" using "local.2.prems" True sorted2 by blast
-    then have "sorted (insert_a x (y # ys))"  by simp
-    then show "sorted (insert_a x (y # ys))" by assumption
+    then have "sorted (insert x (y # ys))"  by simp
+    then show "sorted (insert x (y # ys))" by assumption
   next
     case False
     have "sorted ys" using "local.2.prems" List.linorder_class.sorted.simps(2) by blast
-    also have "sorted (insert_a x ys)" by (simp add: "local.2.hyps" False calculation)
-    moreover have "sorted (y#insert_a x ys)" by (smt "insertion-sort.insert_a.elims" "local.2.prems" False calculation(2) le_cases sorted2)
-    then have "sorted (insert_a x (y # ys))" by (simp add: False)
-    then show "sorted (insert_a x (y # ys))" by assumption
+    also have "sorted (insert x ys)" by (simp add: "local.2.hyps" False calculation)
+    moreover have "sorted (y#insert x ys)" using "local.2.prems" False p_19999 by blast
+    then have "sorted (insert x (y # ys))" by (simp add: False)
+    then show "sorted (insert x (y # ys))" by assumption
   qed
 qed
 
 theorem p_2 : "sorted(insert_sort(ys))"
 proof (induct ys rule:insert_sort.induct)
   case 1
-  have "sorted []"
-    by simp
-  also have "sorted (insert_sort [])"
-    by simp
+  have "sorted []" by simp
+  also have "sorted (insert_sort [])" by simp
   then show ?case by assumption
 next
   case (2 x xs)
-  have "sorted (insert_sort (x # xs)) = sorted(insert_a x (insert_sort(xs)))"
-    by simp
-  also have "sorted(insert_a x (insert_sort(xs)))"
-    by (simp add: "local.2.hyps" p_1)
-  finally show "sorted (insert_sort (x # xs))" by this
+  moreover have "sorted(insert x (insert_sort(xs)))" by (simp add: "local.2.hyps" p_1)
+  then have "sorted (insert_sort (x # xs))" by simp
+  then show "sorted (insert_sort (x # xs))" by assumption
 qed
 
-lemma p_20: "mset (insert_a x ys) = mset (x#ys)"
+lemma p_20: "mset (insert x ys) = mset (x#ys)"
 proof(induct ys arbitrary: x)
   case Nil
   then show ?case  by simp
@@ -76,7 +81,7 @@ qed
 
 fun insert_sort_tail:: "nat list \<Rightarrow> nat list \<Rightarrow> nat list" where
 insert_sort_tail_Nil : "insert_sort_tail [] accum  = accum" |
-insert_sort_tail_Cons: "insert_sort_tail (x#xs) accum  = insert_sort_tail (xs) (insert_a x accum)"
+insert_sort_tail_Cons: "insert_sort_tail (x#xs) accum  = insert_sort_tail (xs) (insert x accum)"
 
 value "insert_sort_tail ([2,4,10]) ([])"
 
